wip

Matroid/Constructions/ClosureAxioms.lean
@@ -4,100 +4,137 @@ import Mathlib.Data.Matroid.IndepAxioms
 
 open Set Matroid
 
-variable {α : Type*} {I J B X : Set α}
+variable {α : Type*} {I J B X Y : Set α} {e : α}
 
 section ClosureMatroid
 
-structure ClosureMatroid (α : Type*) where
+structure PreClosureMatroid (α : Type*) where
   (E : Set α)
   (closure : Set α → Set α)
-  (subset_closure_self : ∀ X ⊆ E, X ⊆ closure X)
-  (closure_subset_closure : ∀ ⦃X Y : Set α⦄, X ⊆ Y → closure X ⊆ closure Y )
-  (closure_closure_eq_closure : ∀ X, closure (closure X) = closure X)
+  (subset_closure_self : ∀ ⦃X⦄, X ⊆ E → X ⊆ closure X)
+  (closure_subset_closure' : ∀ ⦃X Y : Set α⦄, X ⊆ Y → Y ⊆ E → closure X ⊆ closure Y )
+  (closure_closure_eq_closure' : ∀ ⦃X⦄, X ⊆ E → closure (closure X) = closure X)
   (closure_exchange : ∀ ⦃X e f⦄, X ⊆ E → e ∈ E → f ∈ E →
       f ∈ closure (insert e X) \ closure X → e ∈ closure (insert f X) \ X)
+  (closure_inter_inter_ground : ∀ X, closure (X ∩ E) ∩ E = closure X)
   (Indep : Set α → Prop)
   (indep_iff : ∀ ⦃I⦄, Indep I ↔ (∀ e ∈ I, e ∉ closure (I \ {e})) ∧ I ⊆ E)
-  (indep_maximal : ∀ ⦃X⦄, X ⊆ E → ExistsMaximalSubsetProperty Indep X)
-  (closure_inter_inter_ground : ∀ X, closure (X ∩ E) ∩ E = closure X)
 
-namespace ClosureMatroid
 
-lemma closure_subset_ground (M : ClosureMatroid α) (X : Set α) : M.closure X ⊆ M.E := by
+
+-- /-- An auxiliary object corresponding to a matroid as defined by the closure axioms.  -/
+-- structure ClosureMatroid (α : Type*) where
+--   (E : Set α)
+--   (closure : Set α → Set α)
+--   (subset_closure_self : ∀ ⦃X⦄, X ⊆ E → X ⊆ closure X)
+--   (closure_subset_closure' : ∀ ⦃X Y : Set α⦄, X ⊆ Y → Y ⊆ E → closure X ⊆ closure Y )
+--   (closure_closure_eq_closure' : ∀ ⦃X⦄, X ⊆ E → closure (closure X) = closure X)
+--   (closure_exchange : ∀ ⦃X e f⦄, X ⊆ E → e ∈ E → f ∈ E →
+--       f ∈ closure (insert e X) \ closure X → e ∈ closure (insert f X) \ X)
+--   (Indep : Set α → Prop)
+--   (indep_iff : ∀ ⦃I⦄, Indep I ↔ (∀ e ∈ I, e ∉ closure (I \ {e})) ∧ I ⊆ E)
+--   (indep_maximal : ∀ ⦃X⦄, X ⊆ E → ExistsMaximalSubsetProperty Indep X)
+--   (closure_inter_inter_ground : ∀ X, closure (X ∩ E) ∩ E = closure X)
+namespace PreClosureMatroid
+
+variable {M : PreClosureMatroid α}
+
+lemma closure_subset_ground (M : PreClosureMatroid α) (X : Set α) : M.closure X ⊆ M.E := by
   rw [← M.closure_inter_inter_ground]
   apply inter_subset_right
 
-lemma closure_inter_ground (M : ClosureMatroid α) (X : Set α) : M.closure (X ∩ M.E) = M.closure X := by
+lemma closure_inter_ground (M : PreClosureMatroid α) (X : Set α) :
+    M.closure (X ∩ M.E) = M.closure X := by
   rw [← inter_eq_self_of_subset_left (M.closure_subset_ground (X ∩ M.E)),
     M.closure_inter_inter_ground]
 
-lemma Indep.subset_ground {M : ClosureMatroid α} (hI : M.Indep I) : I ⊆ M.E := by
+lemma Indep.subset_ground (hI : M.Indep I) : I ⊆ M.E := by
   rw [indep_iff] at hI
   exact hI.2
 
-lemma Indep.subset {M : ClosureMatroid α} (hJ : M.Indep J) (hIJ : I ⊆ J) : M.Indep I := by
-  rw [M.indep_iff] at *
+lemma closure_subset_closure (M : PreClosureMatroid α) (hXY : X ⊆ Y) :
+    M.closure X ⊆ M.closure Y := by
+  rw [← closure_inter_ground, ← M.closure_inter_ground Y]
+  exact M.closure_subset_closure' (inter_subset_inter_left _ hXY) inter_subset_right
+
+lemma closure_closure_eq_closure (M : PreClosureMatroid α) (X : Set α) :
+    M.closure (M.closure X) = M.closure X := by
+  rw [← M.closure_inter_ground X, closure_closure_eq_closure' _ inter_subset_right]
+
+lemma Indep.subset (hJ : M.Indep J) (hIJ : I ⊆ J) : M.Indep I := by
+  rw [indep_iff] at hJ ⊢
   refine ⟨fun x hxI hx ↦ hJ.1 x (hIJ hxI) ?_, hIJ.trans hJ.2⟩
   exact mem_of_mem_of_subset hx <| M.closure_subset_closure (diff_subset_diff_left hIJ)
 
-lemma Indep.mem_closure_iff {M : ClosureMatroid α} {e : α} (hI : M.Indep I) (he : e ∈ M.E)
+lemma Indep.mem_closure_iff (hI : M.Indep I) (he : e ∈ M.E)
     (heI : e ∉ I) : e ∈ M.closure I ↔ ¬ M.Indep (insert e I) := by
   suffices (e ∉ M.closure I → ∃ x ∈ I, x ∈ M.closure (insert e I \ {x})) → e ∈ M.closure I by
-    simpa (config := { contextual := true }) [M.indep_iff, mem_insert_iff,
+    simpa (config := { contextual := true }) [mem_insert_iff, indep_iff,
       diff_singleton_eq_self heI, insert_subset_iff, he, hI.subset_ground,  iff_def]
 
   simp only [not_imp_comm (a := _ ∈ _), not_exists, not_and]
 
   refine fun h ↦ by_contra fun hcon ↦ hcon <| h fun x hxI hxcl ↦ hcon ?_
-  rw [M.indep_iff] at hI
+  rw [indep_iff] at hI
   rw [← insert_diff_singleton_comm (by rintro rfl; contradiction)] at hxcl
   have hex := M.closure_exchange (X := I \ {x}) (diff_subset.trans hI.2) he
     (M.closure_subset_ground _ hxcl)
   simpa [mem_diff, hxcl, hI.1 x hxI, insert_eq_of_mem hxI, heI] using hex
 
+lemma Indep.aug (hI : M.Indep I) (hInotmax : ¬ Maximal M.Indep I) (hBmax : Maximal M.Indep B) :
+    ∃ e ∈ B \ I, M.Indep (insert e I) := by
+  have hclB : M.closure B = M.E := by
+    refine subset_antisymm (M.closure_subset_ground _) fun y hy ↦ ?_
+    by_cases hyB : y ∈ B
+    · exact M.subset_closure_self hBmax.prop.subset_ground hyB
+    rw [hBmax.prop.mem_closure_iff hy hyB]
+    contrapose! hyB
+    exact hBmax.mem_of_prop_insert hyB
+
+  by_contra! hcon
+
+  have hclI : M.closure I = M.E := by
+    rw [subset_antisymm_iff, and_iff_right (M.closure_subset_ground _), ← hclB,
+      ← M.closure_closure_eq_closure I]
+    refine closure_subset_closure _ fun x hxI' ↦ by_contra fun hxclI ↦ ?_
+    by_cases hxI : x ∈ I
+    · exact hxclI <| M.subset_closure_self hI.subset_ground hxI
+    rw [hI.mem_closure_iff (hBmax.prop.subset_ground hxI') hxI, not_not] at hxclI
+    exact hcon x ⟨hxI', hxI⟩ hxclI
+
+  obtain ⟨y, hyI, hi⟩ := exists_insert_of_not_maximal (fun _ _ h ↦ h.subset) hI hInotmax
+
+  rw [indep_iff, insert_subset_iff] at hi
+  have hy := hi.1 y (by simp)
+  simp only [mem_singleton_iff, insert_diff_of_mem, diff_singleton_eq_self hyI, hclI] at hy
+  exact hy hi.2.1
+
+end PreClosureMatroid
+
+structure ClosureMatroid (α : Type*) extends PreClosureMatroid α where
+  (indep_maximal : ∀ ⦃X⦄, X ⊆ E → ExistsMaximalSubsetProperty Indep X)
+
+namespace ClosureMatroid
+
+variable {M : ClosureMatroid α}
+
 @[simps!] protected def matroid (M : ClosureMatroid α) : Matroid α :=
     IndepMatroid.matroid <| IndepMatroid.mk
   (E := M.E)
   (Indep := M.Indep)
-  (indep_empty := by simp [M.indep_iff])
-  (indep_subset := fun _ _ h ↦ h.subset)
-  (indep_aug := by
-    intro I I' hIindep hInotmax hI'max
-
-    have hclI' : M.closure I' = M.E := by
-      refine subset_antisymm (M.closure_subset_ground _) fun y hy ↦ ?_
-      by_cases hyI' : y ∈ I'
-      · exact M.subset_closure_self _ hI'max.prop.subset_ground hyI'
-      rw [hI'max.prop.mem_closure_iff hy hyI']
-      contrapose! hyI'
-      exact hI'max.mem_of_prop_insert hyI'
-
-    by_contra! hcon
-
-    have hclI : M.closure I = M.E := by
-      rw [subset_antisymm_iff, and_iff_right (M.closure_subset_ground _), ← hclI',
-        ← M.closure_closure_eq_closure I]
-      refine closure_subset_closure _ fun x hxI' ↦ by_contra fun hxclI ↦ ?_
-      by_cases hxI : x ∈ I
-      · exact hxclI <| M.subset_closure_self _ hIindep.subset_ground hxI
-      rw [hIindep.mem_closure_iff (hI'max.prop.subset_ground hxI') hxI, not_not] at hxclI
-      exact hcon x ⟨hxI', hxI⟩ hxclI
-
-    obtain ⟨y, hyI, hi⟩ := exists_insert_of_not_maximal (fun _ _ h ↦ h.subset) hIindep hInotmax
-
-    rw [indep_iff, insert_subset_iff] at hi
-    have hy := hi.1 y (by simp)
-    simp only [mem_singleton_iff, insert_diff_of_mem, diff_singleton_eq_self hyI, hclI] at hy
-    exact hy hi.2.1 )
+  (indep_empty := by simp [M.toPreClosureMatroid.indep_iff])
+  (indep_subset := fun I J hJ hIJ ↦ PreClosureMatroid.Indep.subset hJ hIJ )
+  (indep_aug := fun I B hI hInotmax hBmax ↦ PreClosureMatroid.Indep.aug hI hInotmax hBmax )
   (indep_maximal := fun _ h ↦ M.indep_maximal h)
-  (subset_ground := fun _ ↦ Indep.subset_ground)
+  (subset_ground := fun _ ↦ PreClosureMatroid.Indep.subset_ground)
 
 @[simp] lemma matroid_indep_eq (M : ClosureMatroid α) : M.matroid.Indep = M.Indep := rfl
 
 @[simp] lemma matroid_closure_eq (M : ClosureMatroid α) : M.matroid.closure = M.closure := by
   suffices aux : ∀ X ⊆ M.E, M.matroid.closure X = M.closure X by
     refine funext fun X ↦ ?_
-    rw [← closure_inter_ground, ← Matroid.closure_inter_ground, matroid_E, aux _ (by simp)]
+    rw [← PreClosureMatroid.closure_inter_ground,
+      ← Matroid.closure_inter_ground, matroid_E, aux _ (by simp)]
   refine fun X hX ↦ ?_
   obtain ⟨I, hI⟩ := M.matroid.exists_basis X
   have hi := hI.indep
@@ -106,7 +143,7 @@ lemma Indep.mem_closure_iff {M : ClosureMatroid α} {e : α} (hI : M.Indep I) (h
   refine subset_antisymm ?_ fun e he ↦ ?_
   · simp only [subset_def, hI.indep.mem_closure_iff', matroid_E, matroid_Indep, and_imp]
     refine fun e he h ↦ by_contra fun heX ↦ ?_
-    have heI : e ∉ I := not_mem_subset (hI.subset.trans (M.subset_closure_self X hX)) heX
+    have heI : e ∉ I := not_mem_subset (hI.subset.trans (M.subset_closure_self hX)) heX
     rw [← not_imp_not, ← hi.mem_closure_iff he heI, imp_iff_right heI] at h
     exact heX (M.closure_subset_closure hI.subset h)
   have heE : e ∈ M.E := M.closure_subset_ground X he
@@ -118,10 +155,52 @@ lemma Indep.mem_closure_iff {M : ClosureMatroid α} {e : α} (hI : M.Indep I) (h
   refine mem_of_mem_of_subset he (M.closure_subset_closure fun f hfX ↦ ?_)
   have hfE : f ∈ M.E := hI.subset_ground hfX
   by_cases hfI : f ∈ I
-  · exact M.subset_closure_self _ hi.subset_ground hfI
+  · exact M.subset_closure_self hi.subset_ground hfI
 
   rw [hi.mem_closure_iff hfE hfI]
   contrapose! hfI
   exact hI.mem_of_insert_indep hfX <| by simpa
+
+-- protected def ofFinite (E : Set α) (closure : Set α → Set α)
+--     (subset_closure_self : ∀ ⦃X⦄, X ⊆ E → X ⊆ closure X)
+--     (closure_subset_closure' : ∀ ⦃X Y : Set α⦄, X ⊆ Y → Y ⊆ E → closure X ⊆ closure Y )
+--     (closure_closure_eq_closure' : ∀ ⦃X⦄, X ⊆ E → closure (closure X) = closure X)
+--     (closure_exchange : ∀ ⦃X e f⦄, X ⊆ E → e ∈ E → f ∈ E →
+--       f ∈ closure (insert e X) \ closure X → e ∈ closure (insert f X) \ X)
+--     (exists_finite_closure : ∃ X, X.Finite ∧ E ⊆ closure X)
+--     (closure_inter_inter_ground : ∀ X, closure (X ∩ E) ∩ E = closure X) :
+--     Matroid α := by
+--   let M' : PreClosureMatroid α := {
+--     E := E
+--     closure := closure
+--     subset_closure_self := subset_closure_self
+--     closure_subset_closure' := closure_subset_closure'
+--     closure_closure_eq_closure' := closure_closure_eq_closure'
+--     closure_exchange := closure_exchange
+--     closure_inter_inter_ground := closure_inter_inter_ground
+--     Indep := _
+--     indep_iff := fun _ ↦ Iff.rfl }
+--   have h_fin : ∃ n, ∀ (I : Set α), M'.Indep I → I.encard ≤ ↑n := by
+--     obtain ⟨X, hX, hEX⟩ := exists_finite_closure
+--     refine ⟨X.encard, fun I hI ↦ ?_⟩
+--     rw [PreClosureMatroid.indep_iff] at hI
+--   refine (IndepMatroid.ofBdd E M'.Indep
+--     (by simp) (fun I J hJ hIJ ↦ hJ.subset hIJ) (fun I B hI ↦ hI.aug)
+--     (fun _ ↦ PreClosureMatroid.Indep.subset_ground)
+--     ?_).matroid
+
+
+
+  -- E := E
+  -- closure := closure
+  -- subset_closure_self := subset_closure_self
+  -- closure_subset_closure' := closure_subset_closure'
+  -- closure_closure_eq_closure' := closure_closure_eq_closure'
+  -- closure_exchange := closure_exchange
+  -- Indep I := (∀ e ∈ I, e ∉ closure (I \ {e})) ∧ I ⊆ E
+  -- indep_iff I := Iff.rfl
+  -- indep_maximal := by
+  --   intro X hXE I hI hIX
+  -- closure_inter_inter_ground := closure_inter_inter_ground
 
 end ClosureMatroid
